Metrics/CBULt/CBULt.v
@@ -1,0 +1,20 @@
+Require Import Essentials.Notations.
+Require Import Lattice.CompleteLattice Metrics.UltraMetric
+        Metrics.Mappings Metrics.Complete_UltraMetric.
+Require Import Categories.Category.Category.
+
+Section CBULt.
+  Context (L : CompleteLattice).
+  
+Definition CBULt :=
+  {|
+    Obj := Complete_UltraMetric L;
+    Hom := NonExpansive;
+    compose := @NonExp_compose _;
+    assoc := @NonExp_compose_assoc _;
+    assoc_sym := fun _ _ _ _ _ _ _ => eq_sym (@NonExp_compose_assoc _ _ _ _ _ _ _ _);
+    id := NonExp_id;
+    id_unit_left := @NonExp_id_unit_left _;
+    id_unit_right := @NonExp_id_unit_right _
+  |}
+.
